ongoing: fixing the variability library

src/SPL.lean
@@ -10,19 +10,13 @@ section
 parameters (Feature : Type) [fintype Feature] [decidable_eq Feature]
 
 @[reducible]
-def Config : Type := finset Feature  
-
-@[reducible]
-def ConfigSpace : Type := finset (finset Feature) 
+def Config : Type := finset Feature   
 
 end -- Features and Configurations section
 
 -- Presence Conditions (PCs)
 section 
-parameters {Feature : Type} [fintype Feature] [decidable_eq Feature]
-
-@[reducible]
-def allConfigs : ConfigSpace Feature := finset.univ
+parameters (Feature : Type) [fintype Feature] [decidable_eq Feature]
 
 inductive PC : Type
 | All  : PC 
@@ -32,9 +26,20 @@ inductive PC : Type
 | And  : PC → PC → PC
 | Or   : PC → PC → PC
 
+end
+
+section
+parameters {Feature : Type} [fintype Feature] [decidable_eq Feature]
+
+@[reducible]
+def ConfigSpace : Type := finset (Config Feature)
+
+@[reducible]
+def allConfigs : ConfigSpace := finset.univ
+
 open PC list
 
-def semantics : PC → ConfigSpace Feature
+def semantics : PC Feature → ConfigSpace
 | (All)         := allConfigs
 | (None)        := ∅
 | (Atom f)      := allConfigs.filter (λ p, f ∈ p)
@@ -45,5 +50,126 @@ def semantics : PC → ConfigSpace Feature
 end -- section PCs
 
 notation `⟦` p `⟧` := (semantics p)
+
+-- Var and Lifted
+section
+parameters {Feature : Type} [fintype Feature] [decidable_eq Feature]   
+
+structure Var (α : Type) := (v : α) (pc : PC Feature)
+
+open list 
+
+def disjointPCs {α : Type} (s : list (Var α)) : Prop := 
+    ∀ (c : Config Feature) (x₁ x₂ : Var α), 
+        x₁ ∈ s → x₂ ∈ s → 
+        c ∈ ⟦x₁.pc⟧ → c ∈ ⟦x₂.pc⟧ → x₁ = x₂
+
+def completePCs {α : Type} (s : list (Var α)) : Prop :=
+    ∀ (c : Config Feature), ∃ (v : (Var α)), v ∈ s ∧ c ∈ ⟦v.pc⟧
+
+structure Lifted (α : Type) :=
+    (s    : list (Var α))
+    (disj : disjointPCs s) 
+    (comp : completePCs s)
+
+end -- section Var and Lifted
+
+postfix `↑`:(max+1) := Lifted
+
+-- list_find -- helper for index
+section 
+
+open classical
+
+lemma list_find {α : Type} (q : α → Prop) [decidable_pred q] : 
+    ∀ (l : list α), (∃ y, y ∈ l ∧ q y) → (list.find q l).is_some := 
+begin
+    intros l h₁, 
+    induction l,
+    -- base case
+    apply exists.elim h₁, intros a h₂, apply and.elim h₂, intros h₃ h₄, simp, 
+    apply list.not_mem_nil a h₃,
+    -- induction
+    unfold list.find, cases decidable.em (q l_hd) with hpos hneg,
+    { rw if_pos hpos, simp },
+    { rw if_neg hneg, apply exists.elim h₁, intros a h₂, apply l_ih, apply exists.intro a,
+      simp at h₂, rw and.comm at h₂, rw and_or_distrib_left at h₂, apply or.elim h₂, 
+      {intro h₃, apply and.elim h₃, intros h₄ h₅, rw← h₅ at hneg, contradiction},
+      {intro h₃, rw and.comm, exact h₃}
+    } 
+end
+
+end --section list_find
+
+-- indexing
+section 
+variables {Feature: Type} [fintype Feature] [decidable_eq Feature] {α : Type}
+
+def index'' (v : Lifted α) (ρ : Config Feature) : option (Var α) :=
+    list.find (λ (u: @Var Feature _inst_1 _inst_2 α), ρ ∈ ⟦u.pc⟧) v.s
+
+def configRel (v : Lifted α) (c₁ c₂ : Config Feature) : Prop :=
+    index'' v c₁ = index'' v c₂
+
+lemma configRelReflexive (v : α↑) : ∀ (ρ : Config Feature), configRel v ρ ρ :=
+begin intros ρ, unfold configRel end
+ 
+lemma configRelSymmetric (v: α↑) : 
+    ∀ (c₁ c₂ : Config Feature), configRel v c₁ c₂ → configRel v c₂ c₁ :=
+begin
+    intros c₁ c₂, unfold configRel, intros h, rw h
+end
+
+lemma configRelTransitive (v: α↑) : 
+    ∀ (c₁ c₂ c₃: Config Feature), 
+        configRel v c₁ c₂ → configRel v c₂ c₃ → configRel v c₁ c₃ :=
+begin
+    intros c₁ c₂ c₃, unfold configRel, intros h₁ h₂, rw h₁, rw← h₂
+end
+
+theorem configRel_equiv (α : Type) (v : Lifted α) : @equivalence (Config Feature) (configRel v) := 
+mk_equivalence (configRel v) (configRelReflexive v) (configRelSymmetric v) (configRelTransitive v)
+
+instance lifted_setoid (α : Type) (v : α↑): setoid (Config Feature) :=
+setoid.mk (configRel v) (configRel_equiv α v)
+
+#print lifted_setoid
+
+def index' --[t : fintype Feature] [d : decidable_eq Feature] 
+    (v : Lifted α) (ρ : Config Feature) : Var α :=
+    let pred := λ (u: @Var Feature _inst_1 _inst_2 α), ρ ∈ semantics (u.pc),
+        r    := list.find pred v.s in 
+    if  h : r.is_some 
+    then option.get h
+    else false.elim 
+        begin 
+            apply h, apply (list_find pred v.s (v.comp ρ))
+        end
+
+def index (v : Lifted α) (ρ : Config Feature) : α :=
+    (index' v ρ).v
+
+lemma index_unique (v : Lifted α) (x : Var α) (ρ : Config Feature)  
+    : x ∈ v.s → ρ ∈ semantics (x.pc) → (index'' v ρ) = some x :=
+begin
+    intros h1 h2, 
+    unfold index'',   
+    --generalize_hyp h3 : (hd :: tl) = xs,
+    induction h3 : v.s generalizing x,
+    -- base case
+    rw h3 at h1, simp at h1, contradiction, 
+    -- induction
+    unfold list.find, split_ifs, 
+    apply v.disj, rw h3, simp,
+    exact h1,
+    exact h, 
+    exact h2, 
+    apply ih, 
+
+    --simp, split_ifs, 
+    {rw option.get_of_mem, simp, }
+end
+
+end -- indexing section
 
 end SPL
